src/program_proof/pav/cryptoffi.v
@@ -4,9 +4,9 @@ From Goose.github_com.mit_pdos.pav Require Import cryptoffi.
 Section proof.
 Context `{!heapGS Σ}.
 
-(* Hashing. *)
+(* Hashes. *)
 
-Definition is_hash (data hash : list u8) : iProp Σ.
+Definition is_hash (data hash : list w8) : iProp Σ.
 Proof. Admitted.
 
 #[global]
@@ -31,69 +31,69 @@ Proof. Admitted.
 
 Lemma wp_Hash sl_data data :
   {{{
-    "Hdata" ∷ own_slice_small sl_data byteT 1 data
+    "Hdata" ∷ own_slice_small sl_data byteT (DfracOwn 1) data
   }}}
   Hash (slice_val sl_data)
   {{{
     sl_hash hash, RET (slice_val sl_hash);
-    "Hdata" ∷ own_slice_small sl_data byteT 1 data ∗
-    "Hhash" ∷ own_slice_small sl_hash byteT 1 hash ∗
+    "Hdata" ∷ own_slice_small sl_data byteT (DfracOwn 1) data ∗
+    "Hhash" ∷ own_slice_small sl_hash byteT (DfracOwn 1) hash ∗
     "#His_hash" ∷ is_hash data hash
   }}}.
 Proof. Admitted.
 
-(* Signing and verifying. *)
+(* Signatures. *)
 
-Definition own_sk (sk : Slice.t) (P : list u8 → iProp Σ) (hon : bool) : iProp Σ.
+Definition own_sk (sk : Slice.t) (P : list w8 → iProp Σ) (hon : bool) : iProp Σ.
 Admitted.
 
-Definition is_pk (pk : Slice.t) (P : list u8 → iProp Σ) (hon : bool) : iProp Σ.
+Definition is_pk (pk : Slice.t) (P : list w8 → iProp Σ) (hon : bool) : iProp Σ.
 Admitted.
 
 #[global]
 Instance is_pk_persistent pk P hon : Persistent (is_pk pk P hon).
 Proof. Admitted.
 
-Lemma wp_MakeKeys P hon :
+Lemma wp_GenerateKey P hon :
   {{{
     "%Hpersis" ∷ ⌜∀ l, Persistent (P l)⌝
   }}}
-  MakeKeys #()
+  GenerateKey #()
   {{{
-    sk pk, RET ((slice_val sk), (slice_val pk));
-    "Hsk" ∷ own_sk sk P hon ∗
-    "#Hpk" ∷ is_pk pk P hon
+    pk sk, RET ((slice_val pk), (slice_val sk));
+    "#Hpk" ∷ is_pk pk P hon ∗
+    "Hsk" ∷ own_sk sk P hon
   }}}.
 Proof. Admitted.
 
-Lemma wp_Sign sk P hon sl_data data :
+Lemma wp_Sign sk P hon sl_msg msg :
   {{{
     "Hsk" ∷ own_sk sk P hon ∗
-    "HP" ∷ P data ∗
-    "Hdata" ∷ own_slice_small sl_data byteT 1 data
+    "HP" ∷ P msg ∗
+    "Hmsg" ∷ own_slice_small sl_msg byteT (DfracOwn 1) msg
   }}}
-  Sign (slice_val sk) (slice_val sl_data)
+  PrivateKey__Sign (slice_val sk) (slice_val sl_msg)
   {{{
-    sl_sig (sig : list u8), RET (slice_val sl_sig);
+    sl_sig (sig : list w8), RET (slice_val sl_sig);
     "Hsk" ∷ own_sk sk P hon ∗
-    "Hdata" ∷ own_slice_small sl_data byteT 1 data ∗
-    "Hsig" ∷ own_slice_small sl_sig byteT 1 sig
+    "Hmsg" ∷ own_slice_small sl_msg byteT (DfracOwn 1) msg ∗
+    "Hsig" ∷ own_slice_small sl_sig byteT (DfracOwn 1) sig
   }}}.
 Proof. Admitted.
 
-Lemma wp_Verify pk P hon sl_sig (sig : list u8) sl_data (data : list u8) :
+Lemma wp_Verify pk P hon sl_sig (sig : list w8) sl_msg (msg : list w8) :
   {{{
     "#Hpk" ∷ is_pk pk P hon ∗
-    "Hsig" ∷ own_slice_small sl_sig byteT 1 sig ∗
-    "Hdata" ∷ own_slice_small sl_data byteT 1 data
+    "Hsig" ∷ own_slice_small sl_sig byteT (DfracOwn 1) sig ∗
+    "Hmsg" ∷ own_slice_small sl_msg byteT (DfracOwn 1) msg
   }}}
-  Verify (slice_val pk) (slice_val sl_data) (slice_val sl_sig)
+  PublicKey__Verify (slice_val pk) (slice_val sl_msg) (slice_val sl_sig)
   {{{
     (err : bool), RET #err;
-    "Hsig" ∷ own_slice_small sl_sig byteT 1 sig ∗
-    "Hdata" ∷ own_slice_small sl_data byteT 1 data ∗
+    "Hsig" ∷ own_slice_small sl_sig byteT (DfracOwn 1) sig ∗
+    "Hmsg" ∷ own_slice_small sl_msg byteT (DfracOwn 1) msg ∗
     if negb err && hon then
-      "HP" ∷ P data
+      "HP" ∷ P msg
     else True%I
   }}}.
 Proof. Admitted.
