src/program_proof/pav/merkle.v
@@ -1,7 +1,7 @@
 From Perennial.program_proof Require Import grove_prelude.
 From Goose.github_com.mit_pdos.pav Require Import merkle.
 
-From Perennial.program_proof.pav.merkle Require Import shim.
+From Perennial.program_proof.pav Require Import common cryptoffi cryptoutil.
 From Perennial.program_proof Require Import std_proof.
 
 Section defs.
@@ -9,12 +9,12 @@ Context `{!heapGS Σ}.
 
 Inductive tree : Type :=
   (* Cut only exists for proof checking trees. *)
-  | Cut : list u8 → tree
+  | Cut : list w8 → tree
   | Empty : tree
-  | Leaf : list u8 → tree
+  | Leaf : list w8 → tree
   | Interior : list tree → tree.
 
-Fixpoint containsNodeAtEnd (tr : tree) (id : list u8) (node : tree) : Prop :=
+Fixpoint containsNodeAtEnd (tr : tree) (id : list w8) (node : tree) : Prop :=
   match tr with
   | Cut _ => False
   | Empty => id = [] ∧ tr = node
@@ -23,17 +23,17 @@ Fixpoint containsNodeAtEnd (tr : tree) (id : list u8) (node : tree) : Prop :=
     match id with
     | [] => False
     | pos :: rest =>
-      ∃ child, children !! uint.nat pos = Some child ∧ containsNodeAtEnd child rest node
+      ∃ child, children !! Z.to_nat (word.unsigned pos) = Some child ∧ containsNodeAtEnd child rest node
     end
   end.
 
-Fixpoint is_tree_hash (tr : tree) (hash : list u8) : iProp Σ :=
+Fixpoint is_tree_hash (tr : tree) (hash : list w8) : iProp Σ :=
   match tr with
   | Cut hash' => ⌜hash = hash' ∧ length hash' = 32%nat⌝
   | Empty => is_hash [W8 0] hash
   | Leaf val => is_hash (val ++ [W8 1]) hash
   | Interior children =>
-    ∃ (child_hashes : list (list u8)),
+    ∃ (child_hashes : list (list w8)),
     let map_fn := (λ c h, is_tree_hash c h) in
     ([∗ list] child_fn;hash' ∈ (map_fn <$> children);child_hashes,
       child_fn hash') ∗
@@ -187,7 +187,7 @@ Proof.
   }
 Qed.
 
-Definition own_Node' (recur : loc -d> tree -d> iPropO Σ) : loc -d> tree -d> iPropO Σ :=
+Definition own_node' (recur : loc -d> tree -d> iPropO Σ) : loc -d> tree -d> iPropO Σ :=
   (λ ptr_tr tr,
     match tr with
     (* We should never have cuts in in-memory trees. *)
@@ -198,35 +198,35 @@ Definition own_Node' (recur : loc -d> tree -d> iPropO Σ) : loc -d> tree -d> iPr
       "%Hnil" ∷ ⌜ptr_tr = null⌝
     | Leaf val =>
       ∃ sl_val hash sl_hash,
-      "Hval" ∷ own_slice_small sl_val byteT 1 val ∗
-      "Hptr_val" ∷ ptr_tr ↦[Node :: "Val"] (slice_val sl_val) ∗
+      "Hval" ∷ own_slice_small sl_val byteT (DfracOwn 1) val ∗
+      "Hptr_val" ∷ ptr_tr ↦[node :: "Val"] (slice_val sl_val) ∗
       "#His_hash" ∷ is_tree_hash tr hash ∗
-      "Hhash" ∷ own_slice_small sl_hash byteT 1 hash ∗
-      "Hsl_hash" ∷ ptr_tr ↦[Node :: "hash"] (slice_val sl_hash)
+      "Hhash" ∷ own_slice_small sl_hash byteT (DfracOwn 1) hash ∗
+      "Hsl_hash" ∷ ptr_tr ↦[node :: "hash"] (slice_val sl_hash)
     | Interior children =>
       ∃ hash sl_hash sl_children ptr_children,
       "#His_hash" ∷ is_tree_hash tr hash ∗
-      "Hhash" ∷ own_slice_small sl_hash byteT 1 hash ∗
-      "Hsl_children" ∷ own_slice_small sl_children ptrT 1 ptr_children ∗
-      "Hptr_children" ∷ ptr_tr ↦[Node :: "Children"] (slice_val sl_children) ∗
+      "Hhash" ∷ own_slice_small sl_hash byteT (DfracOwn 1) hash ∗
+      "Hsl_children" ∷ own_slice_small sl_children ptrT (DfracOwn 1) ptr_children ∗
+      "Hptr_children" ∷ ptr_tr ↦[node :: "Children"] (slice_val sl_children) ∗
       "Hchildren" ∷
         ([∗ list] child;ptr_child ∈ children;ptr_children,
           ▷ recur ptr_child child)
     end)%I.
 
-Local Instance own_Node'_contractive : Contractive own_Node'.
+Local Instance own_node'_contractive : Contractive own_node'.
 Proof. solve_contractive. Qed.
 
-Definition own_Node : loc → tree → iProp Σ := fixpoint own_Node'.
+Definition own_node : loc → tree → iProp Σ := fixpoint own_node'.
 
-Lemma own_Node_unfold ptr obj :
-  own_Node ptr obj ⊣⊢ (own_Node' own_Node) ptr obj.
+Lemma own_node_unfold ptr obj :
+  own_node ptr obj ⊣⊢ (own_node' own_node) ptr obj.
 Proof.
-  apply (fixpoint_unfold own_Node').
+  apply (fixpoint_unfold own_node').
 Qed.
 
-Definition tree_to_map (tr : tree) : gmap (list u8) (list u8) :=
-  let fix traverse (tr : tree) (acc : gmap (list u8) (list u8)) (id : list u8) :=
+Definition tree_to_map (tr : tree) : gmap (list w8) (list w8) :=
+  let fix traverse (tr : tree) (acc : gmap (list w8) (list w8)) (id : list w8) :=
     match tr with
     | Cut _ => acc
     | Empty => acc
@@ -234,7 +234,7 @@ Definition tree_to_map (tr : tree) : gmap (list u8) (list u8) :=
     | Interior children =>
       (* Grab all entries from the children, storing the ongoing id. *)
       (foldr
-        (λ child (pIdxAcc:(Z * gmap (list u8) (list u8))),
+        (λ child (pIdxAcc:(Z * gmap (list w8) (list w8))),
           let acc' := traverse child pIdxAcc.2 (id ++ [W8 pIdxAcc.1])
           in (pIdxAcc.1 + 1, acc'))
         (0, acc) children
@@ -244,84 +244,68 @@ Definition tree_to_map (tr : tree) : gmap (list u8) (list u8) :=
 
 Definition own_Tree ptr_tr entry_map : iProp Σ :=
   ∃ tr root,
-  "Hnode" ∷ own_Node root tr ∗
+  "Hnode" ∷ own_node root tr ∗
   "%Htree_map" ∷ ⌜tree_to_map tr = entry_map⌝ ∗
   "Hptr_root" ∷ ptr_tr ↦[Tree :: "Root"] #root.
 
-(* Note: make everything RO for easy big sep logic. *)
-Definition is_Slice2D (sl_dim0 : Slice.t) (obj_dim0 : list (list u8)) : iProp Σ :=
-  ∃ list_dim0,
-  "#Hro_sl_dim0" ∷ readonly (own_slice_small sl_dim0 (slice.T byteT) 1 list_dim0) ∗
-  "#Hsep_dim0" ∷ ([∗ list] sl_dim1;obj_dim1 ∈ list_dim0;obj_dim0,
-    "#Hro_sl_dim1" ∷ readonly (own_slice_small sl_dim1 byteT 1 obj_dim1)).
-
-Definition is_Slice3D (sl_dim0 : Slice.t) (obj_dim0 : list (list (list u8))) : iProp Σ :=
-  ∃ list_dim0,
-  "#Hro_sl_dim0" ∷ readonly (own_slice_small sl_dim0 (slice.T (slice.T byteT)) 1 list_dim0) ∗
-  "#Hsep_dim0" ∷ ([∗ list] sl_dim1;obj_dim1 ∈ list_dim0;obj_dim0,
-    ∃ list_dim1,
-    "#Hro_sl_dim1" ∷ readonly (own_slice_small sl_dim1 (slice.T byteT) 1 list_dim1) ∗
-    "#Hsep_dim1" ∷ ([∗ list] sl_dim2;obj_dim2 ∈ list_dim1;obj_dim1,
-      "#Hro_sl_dim2" ∷ readonly (own_slice_small sl_dim2 byteT 1 obj_dim2))).
-
 End defs.
 
-Module PathProof.
+Module pathProof.
 Record t :=
   mk {
-    Id: list u8;
-    NodeHash: list u8;
-    Digest: list u8;
-    ChildHashes: list (list (list u8));
+    id: list w8;
+    nodeHash: list w8;
+    digest: list w8;
+    childHashes: list (list (list w8));
   }.
 
 Section local_defs.
 Context `{!heapGS Σ}.
 Definition own (ptr : loc) (obj : t) : iProp Σ :=
-  ∃ sl_Id sl_NodeHash sl_Digest sl_ChildHashes,
-  "HId" ∷ own_slice_small sl_Id byteT 1 obj.(Id) ∗
-  "Hptr_Id" ∷ ptr ↦[PathProof :: "Id"] (slice_val sl_Id) ∗
-  "HNodeHash" ∷ own_slice_small sl_NodeHash byteT 1 obj.(NodeHash) ∗
-  "Hptr_NodeHash" ∷ ptr ↦[PathProof :: "NodeHash"] (slice_val sl_NodeHash) ∗
-  "HDigest" ∷ own_slice_small sl_Digest byteT 1 obj.(Digest) ∗
-  "Hptr_Digest" ∷ ptr ↦[PathProof :: "Digest"] (slice_val sl_Digest) ∗
-  "#HChildHashes" ∷ is_Slice3D sl_ChildHashes obj.(ChildHashes) ∗
-  "Hptr_ChildHashes" ∷ ptr ↦[PathProof :: "ChildHashes"] (slice_val sl_ChildHashes) ∗
-  "%Hlen_id_depth" ∷ ⌜length obj.(Id) = length obj.(ChildHashes)⌝ ∗
-  "%Hlen_id_ub" ∷ ⌜length obj.(Id) ≤ 32⌝.
+  ∃ sl_id sl_nodeHash sl_digest sl_childHashes,
+  "Hid" ∷ own_slice_small sl_id byteT (DfracOwn 1) obj.(id) ∗
+  "Hptr_id" ∷ ptr ↦[pathProof :: "id"] (slice_val sl_id) ∗
+  "HnodeHash" ∷ own_slice_small sl_nodeHash byteT (DfracOwn 1) obj.(nodeHash) ∗
+  "Hptr_nodeHash" ∷ ptr ↦[pathProof :: "nodeHash"] (slice_val sl_nodeHash) ∗
+  "Hdigest" ∷ own_slice_small sl_digest byteT (DfracOwn 1) obj.(digest) ∗
+  "Hptr_digest" ∷ ptr ↦[pathProof :: "digest"] (slice_val sl_digest) ∗
+  "#HchildHashes" ∷ is_Slice3D sl_childHashes obj.(childHashes) ∗
+  "Hptr_childHashes" ∷ ptr ↦[pathProof :: "childHashes"] (slice_val sl_childHashes) ∗
+  "%Hlen_id_depth" ∷ ⌜length obj.(id) = length obj.(childHashes)⌝ ∗
+  "%Hlen_id_ub" ∷ ⌜length obj.(id) ≤ 32⌝.
 End local_defs.
-End PathProof.
+End pathProof.
 
 Section proofs.
 Context `{!heapGS Σ}.
 
-Lemma wp_Put ptr_tr entry_map sl_id id sl_val val :
+Lemma wp_Tree_Put ptr_tr entry_map sl_id id sl_val val :
   {{{
     "Htree" ∷ own_Tree ptr_tr entry_map ∗
-    "Hid" ∷ own_slice_small sl_id byteT 1 id ∗
-    "Hval" ∷ own_slice_small sl_val byteT 1 val
+    "Hid" ∷ own_slice_small sl_id byteT (DfracOwn 1) id ∗
+    "Hval" ∷ own_slice_small sl_val byteT (DfracOwn 1) val
   }}}
   Tree__Put #ptr_tr (slice_val sl_id) (slice_val sl_val)
   {{{
-    sl_digest ptr_proof (err : u64),
+    sl_digest ptr_proof (err : bool),
     RET ((slice_val sl_digest), #ptr_proof, #err);
-    if bool_decide (err = 0) then
+    if negb err then
       "Htree" ∷ own_Tree ptr_tr (<[id:=val]>entry_map)
     else True%I
   }}}.
 Proof. Admitted.
 
-Lemma wp_NodeHashNull :
+Lemma wp_node_getHash_null :
   {{{ True }}}
-  Node__Hash #null
+  node__getHash #null
   {{{
     sl_hash hash, RET (slice_val sl_hash);
-    "Hhash" ∷ own_slice_small sl_hash byteT 1 hash ∗
+    "Hhash" ∷ own_slice_small sl_hash byteT (DfracOwn 1) hash ∗
     "#His_hash" ∷ is_tree_hash Empty hash
   }}}.
 Proof.
   iIntros (Φ) "_ HΦ".
-  rewrite /Node__Hash.
+  rewrite /node__getHash.
   wp_apply wp_SliceSingleton; [val_ty|];
     iIntros (sl_data) "Hdata".
   wp_apply (wp_Hash with "[Hdata]").
@@ -336,51 +320,11 @@ Proof.
   iFrame "#∗".
 Qed.
 
-Lemma wp_HasherWrite sl_hr hr ptr_hr sl_data (data : list u8) :
-  {{{
-    "Hhr" ∷ own_slice_small sl_hr byteT 1 hr ∗
-    "Hptr_hr" ∷ ptr_hr ↦[slice.T byteT] (slice_val sl_hr) ∗
-    "#Hdata" ∷ readonly (own_slice_small sl_data byteT 1 data)
-  }}}
-  HasherWrite #ptr_hr (slice_val sl_data)
-  {{{
-    sl_hr', RET #();
-    "Hhr" ∷ own_slice_small sl_hr' byteT 1 (hr ++ data) ∗
-    "Hptr_hr" ∷ ptr_hr ↦[slice.T byteT] (slice_val sl_hr')
-  }}}.
-Proof. Admitted.
-
-Lemma wp_HasherWriteSl sl_hr hr ptr_hr sl_data data :
-  {{{
-    "Hhr" ∷ own_slice_small sl_hr byteT 1 hr ∗
-    "Hptr_hr" ∷ ptr_hr ↦[slice.T byteT] (slice_val sl_hr) ∗
-    "#Hdata" ∷ is_Slice2D sl_data data
-  }}}
-  HasherWriteSl #ptr_hr (slice_val sl_data)
-  {{{
-    sl_hr', RET #();
-    "Hhr" ∷ own_slice_small sl_hr' byteT 1 (hr ++ concat data) ∗
-    "Hptr_hr" ∷ ptr_hr ↦[slice.T byteT] (slice_val sl_hr')
-  }}}.
-Proof. Admitted.
-
-Lemma wp_HasherSumNil sl_hr hr :
-  {{{
-    "Hhr" ∷ own_slice_small sl_hr byteT 1 hr
-  }}}
-  HasherSum (slice_val sl_hr) slice.nil
-  {{{
-    sl_hash hash, RET (slice_val sl_hash);
-    "#Hhash" ∷ is_hash hr hash ∗
-    "Hsl_hash" ∷ own_slice_small sl_hash byteT 1 hash
-  }}}.
-Proof. Admitted.
-
-Lemma wp_IsValidHashSl sl_data data :
+Lemma wp_isValidHashSl sl_data data :
   {{{
     "#Hdata" ∷ is_Slice2D sl_data data
   }}}
-  IsValidHashSl (slice_val sl_data)
+  isValidHashSl (slice_val sl_data)
   {{{
     (ok : bool), RET #ok;
     if bool_decide ok then
@@ -389,25 +333,25 @@ Lemma wp_IsValidHashSl sl_data data :
   }}}.
 Proof. Admitted.
 
-Lemma wp_PathProofCheck ptr_proof proof val :
+Lemma wp_pathProof_check ptr_proof proof val :
   {{{
-    "Hproof" ∷ PathProof.own ptr_proof proof ∗
+    "Hproof" ∷ pathProof.own ptr_proof proof ∗
     let node := match val with
     | None => Empty
     | Some val' => Leaf val'
     end in
-    "Hhash" ∷ is_tree_hash node proof.(PathProof.NodeHash)
+    "Hhash" ∷ is_tree_hash node proof.(pathProof.nodeHash)
   }}}
-  PathProof__Check #ptr_proof
+  pathProof__check #ptr_proof
   {{{
-    (err : u64), RET #err;
-    if bool_decide (err = 0) then
-      "Hpath" ∷ is_path_val proof.(PathProof.Id) val proof.(PathProof.Digest)
+    (err : bool), RET #err;
+    if negb err then
+      "Hpath" ∷ is_path_val proof.(pathProof.id) val proof.(pathProof.digest)
     else True%I
   }}}.
 Proof.
   iIntros (Φ) "H HΦ"; iNamed "H"; iNamed "Hproof".
-  rewrite /PathProof__Check.
+  rewrite /pathProof__check.
   wp_apply wp_ref_to; [val_ty|];
     iIntros (ptr_err) "Hptr_err".
   wp_loadField.
@@ -415,30 +359,28 @@ Proof.
   wp_loadField.
   wp_apply wp_slice_len.
   wp_apply wp_ref_to; [val_ty|]; iIntros (ptr_loopIdx) "HloopIdx".
-  iDestruct ("HChildHashes") as (?) "H"; iNamed "H".
-  iMod (readonly_alloc_1 with "HNodeHash") as "#Hro_NodeHash".
-  iDestruct (big_sepL2_length with "Hsep_dim0") as "%Hlen_ChildHashes".
-  iMod (readonly_load with "Hro_sl_dim0") as (q) "H";
-    iDestruct (own_slice_small_sz with "H") as "%Hlen_list_dim0";
-    iClear (q) "H".
+  iDestruct ("HchildHashes") as (?) "H"; iNamed "H".
+  iMod (own_slice_small_persist with "HnodeHash") as "#HnodeHash".
+  iDestruct (big_sepL2_length with "Hsep_dim0") as "%Hlen_childHashes".
+  iDestruct (own_slice_small_sz with "Hsl_dim0") as "%Hlen_list_dim0".
 
   (* Entering the main loop. *)
   set for_inv :=
-    (λ loopIdx, ∃ sl_currHash currHash (err : u64),
-      "HId" ∷ own_slice_small sl_Id byteT 1 proof.(PathProof.Id) ∗
-      "Hptr_Id" ∷ ptr_proof ↦[PathProof :: "Id"] sl_Id ∗
-      "Hptr_ChildHashes" ∷ ptr_proof ↦[PathProof :: "ChildHashes"] sl_ChildHashes ∗
-      "#Hro_sl_currHash" ∷ readonly (own_slice_small sl_currHash byteT 1 currHash) ∗
+    (λ loopIdx, ∃ sl_currHash currHash (err : bool),
+      "Hid" ∷ own_slice_small sl_id byteT (DfracOwn 1) proof.(pathProof.id) ∗
+      "Hptr_id" ∷ ptr_proof ↦[pathProof :: "id"] sl_id ∗
+      "Hptr_childHashes" ∷ ptr_proof ↦[pathProof :: "childHashes"] sl_childHashes ∗
+      "#Hsl_currHash" ∷ own_slice_small sl_currHash byteT DfracDiscarded currHash ∗
       "Hptr_currHash" ∷ ptr_currHash ↦[slice.T byteT] sl_currHash ∗
-      "Hptr_err" ∷ ptr_err ↦[uint64T] #err ∗
-      "Herr_pred" ∷ if bool_decide (err = 0) then
+      "Hptr_err" ∷ ptr_err ↦[boolT] #err ∗
+      "Herr_pred" ∷ if negb err then
         "Hpath_val" ∷ is_path_val
-          (drop (length proof.(PathProof.Id) - uint.nat loopIdx)
-          proof.(PathProof.Id)) val currHash
-      else True)%I : u64 → iProp Σ.
-  wp_apply (wp_forUpto for_inv with "[] [$HId $Hptr_Id $Hptr_ChildHashes $HloopIdx $HcurrHash $Hro_NodeHash $Hptr_err Hhash]"); [word|..].
+          (drop (length proof.(pathProof.id) - (Z.to_nat (word.unsigned loopIdx)))
+          proof.(pathProof.id)) val currHash
+      else True)%I : w64 → iProp Σ.
+  wp_apply (wp_forUpto for_inv with "[] [$Hid $Hptr_id $Hptr_childHashes $HloopIdx $HcurrHash $HnodeHash $Hptr_err Hhash]"); [word|..].
   2: {
-    assert ((length proof.(PathProof.Id) - uint.nat 0)%nat = length proof.(PathProof.Id)) as H by word;
+    assert ((length proof.(pathProof.id) - 0%nat)%nat = length proof.(pathProof.id)) as H by word;
       iEval (rewrite H); clear H.
     iEval (rewrite drop_all).
     iFrame.
@@ -449,11 +391,11 @@ Proof.
     iIntros (loopIdx Φ2) "!> (Hinv & HloopIdx & %HloopBound) HΦ2";
       iNamed "Hinv".
     wp_load.
-    wp_apply (wp_loadField with "[$Hptr_ChildHashes]");
-      iIntros "Hptr_ChildHashes".
+    wp_apply (wp_loadField with "[$Hptr_childHashes]");
+      iIntros "Hptr_childHashes".
 
     (* Note: move all the sep fetches into one block, like this. *)
-    iMod (readonly_load with "Hro_sl_dim0") as (?) "Hsl_dim0".
+    (* TODO: change all uint out of backwords compat thing *)
     assert (∃ (sl_dim1' : Slice.t),
       list_dim0 !! uint.nat (length list_dim0 - 1 - uint.nat loopIdx) =
       Some sl_dim1') as [sl_dim1' Hlook_sl_dim1'].
@@ -461,37 +403,35 @@ Proof.
     iDestruct (big_sepL2_lookup_1_some with "Hsep_dim0") as %[obj_dim1' Hlook_obj_dim1']; [done|].
     iDestruct (big_sepL2_lookup with "Hsep_dim0") as (list_dim1') "H";
       [done..|]; iNamed "H".
-    iMod (readonly_load with "Hro_sl_dim1") as (?) "Hsl_dim1".
     iDestruct (own_slice_small_sz with "Hsl_dim1") as "%Hlen_list_dim1'".
     iDestruct (big_sepL2_length with "Hsep_dim1") as "%Hlen_obj_dim1'".
-    iDestruct (own_slice_small_sz with "HId") as "%Hlen_Id".
+    iDestruct (own_slice_small_sz with "Hid") as "%Hlen_id".
 
     (* Rewrite this early since it appears in multiple sub-terms. *)
-    replace (word.sub (word.sub sl_ChildHashes.(Slice.sz) 1) loopIdx) with
+    replace (word.sub (word.sub sl_childHashes.(Slice.sz) 1) loopIdx) with
       (W64 (length list_dim0 - 1 - uint.nat loopIdx)) by word.
 
-    wp_apply (wp_SliceGet with "[$Hsl_dim0]"); [done|];
-      iIntros "Hsl_dim0".
+    wp_apply (wp_SliceGet with "[$Hsl_dim0]"); [done|]; iIntros "_".
     wp_apply wp_slice_len.
 
     wp_if_destruct.
     { wp_store. iApply "HΦ2". by iFrame "#∗". }
     replace (word.sub 256 1) with (W64 255) in Heqb;
       [|word]; rename Heqb into Hsz_sl_dim1'.
-    wp_apply (wp_IsValidHashSl with "[$Hro_sl_dim1 $Hsep_dim1]").
+    wp_apply (wp_isValidHashSl with "[$Hsl_dim1 $Hsep_dim1]").
       iIntros (ok) "H".
     wp_if_destruct.
     { wp_store. iApply "HΦ2". by iFrame "#∗". }
     iSimpl in "H"; iNamed "H"; rename Hlen into Hhash_len_obj_dim1'.
 
-    wp_apply (wp_loadField with "[$Hptr_Id]");
-      iIntros "Hptr_Id".
-    assert (∃ (pos : u8),
-      proof.(PathProof.Id) !! uint.nat (length list_dim0 - 1 - uint.nat loopIdx) =
+    wp_apply (wp_loadField with "[$Hptr_id]");
+      iIntros "Hptr_id".
+    assert (∃ (pos : w8),
+      proof.(pathProof.id) !! uint.nat (length list_dim0 - 1 - uint.nat loopIdx) =
       Some pos) as [pos Hlook_pos].
     { apply lookup_lt_is_Some. word. }
-    wp_apply (wp_SliceGet with "[$HId]"); [done|];
-      iIntros "HId".
+    wp_apply (wp_SliceGet with "[$Hid]"); [done|];
+      iIntros "Hid".
 
     (* TODO: word should know this. *)
     assert (length list_dim1' = 255%nat) as H255_list_dim1'.
@@ -501,7 +441,7 @@ Proof.
 
     (* The complicated slice splitting logic. *)
     iDestruct (own_slice_small_wf with "Hsl_dim1") as "%Hwf_sl_dim1".
-    iDestruct (slice_small_split _ (u8_to_u64 pos) with "Hsl_dim1") as "[Hsl_before Hsl_after]".
+    iDestruct (slice_small_split _ (W64 (word.unsigned pos)) with "Hsl_dim1") as "[Hsl_before Hsl_after]".
     (* TODO: word should know this. *)
     { rewrite u8_to_u64_Z. lia. }
     wp_apply wp_SliceTake.
@@ -510,15 +450,12 @@ Proof.
     { rewrite u8_to_u64_Z. lia. }
     iEval (rewrite u8_to_u64_Z) in "Hsl_before".
     iEval (rewrite u8_to_u64_Z) in "Hsl_after".
-    (* TODO: we really shouldn't need to type in the entire P here. *)
-    iMod (readonly_alloc (own_slice_small (slice_take sl_dim1' (u8_to_u64 pos)) (slice.T byteT) 1 (take (uint.nat pos) list_dim1')) with "[$Hsl_before]") as "#Hro_sl_before".
-    iMod (readonly_alloc (own_slice_small (slice_skip sl_dim1' (slice.T byteT) (u8_to_u64 pos)) (slice.T byteT) 1 (drop (uint.nat pos) list_dim1')) with "[$Hsl_after]") as "#Hro_sl_after".
 
     wp_apply wp_ref_of_zero; [done|];
       iIntros (ptr_hr) "Hptr_hr".
     iEval (rewrite zero_slice_val) in "Hptr_hr".
-    iDestruct (own_slice_small_nil byteT 1 (Slice.nil)) as "Hnil"; [done|].
-    wp_apply (wp_HasherWriteSl with "[$Hptr_hr $Hnil $Hro_sl_before]").
+    iDestruct (own_slice_small_nil byteT (DfracOwn 1) (Slice.nil)) as "Hnil"; [done|].
+    wp_apply (wp_HasherWriteSl with "[$Hptr_hr $Hnil $Hsl_before]").
     {
       iApply big_sepL2_prefix.
       4: iFrame "#".
@@ -528,9 +465,9 @@ Proof.
     }
     iIntros (sl_hr) "H"; iNamed "H".
     wp_load.
-    wp_apply (wp_HasherWrite with "[$Hptr_hr $Hhr $Hro_sl_currHash]");
+    wp_apply (wp_HasherWrite with "[$Hptr_hr $Hhr $Hsl_currHash]");
       clear sl_hr; iIntros (sl_hr) "H"; iNamed "H".
-    wp_apply (wp_HasherWriteSl with "[$Hptr_hr $Hhr $Hro_sl_after]").
+    wp_apply (wp_HasherWriteSl with "[$Hptr_hr $Hhr $Hsl_after]").
     {
       iApply big_sepL2_suffix.
       4: iFrame "#".
@@ -543,26 +480,21 @@ Proof.
       iIntros (sl_tag) "H";
       iDestruct (slice.own_slice_to_small with "H") as "Hsl_tag".
     iAssert (own_slice_small _ _ _ [W8 2]) with "Hsl_tag" as "Hsl_tag".
-    iMod (readonly_alloc_1 with "Hsl_tag") as "#Hro_sl_tag".
-    wp_apply (wp_HasherWrite with "[$Hptr_hr $Hhr $Hro_sl_tag]").
+    iMod (own_slice_small_persist with "Hsl_tag") as "#Hsl_tag".
+    wp_apply (wp_HasherWrite with "[$Hptr_hr $Hhr $Hsl_tag]").
     clear sl_hr; iIntros (sl_hr) "H"; iNamed "H".
     wp_load.
     wp_apply (wp_HasherSumNil with "Hhr");
       iIntros (sl_hash hash) "H"; iNamed "H".
     wp_store.
-    iMod (readonly_alloc_1 with "Hsl_hash") as "#Hro_sl_hash".
-    iClear (sl_tag) "Hro_NodeHash Hro_sl_before Hro_sl_after Hnil Hro_sl_tag".
+    iMod (own_slice_small_persist with "Hsl_hash") as "#Hsl_hash".
+    iClear (sl_tag) "HnodeHash Hsl_before Hsl_after Hnil Hsl_tag".
 
     (* Done with code, now re-establish loop inv. *)
-    case_bool_decide; rename H into Herr; iNamed "Herr_pred".
-    2: { iApply "HΦ2". iFrame "#∗". by case_bool_decide. }
-    iApply "HΦ2".
-    iFrame "#∗".
-    case_bool_decide; [|done].
-    clear Herr H.
 
+    destruct err; iNamed "Herr_pred"; iApply "HΦ2"; iFrame "#∗"; [done|].
     rewrite /is_path_val.
-    iDestruct "Hpath_val" as (tr) "[Htr_hash %Htr_contains]".
+    iDestruct "Herr_pred" as "[Htr_hash %Htr_contains]".
     iExists (Interior (
       ((λ h, Cut h) <$> (take (uint.nat pos) obj_dim1')) ++
       [tr] ++
@@ -606,8 +538,8 @@ Proof.
     rewrite (drop_S _ pos _ _).
     2: { rewrite <-Hlook_pos. f_equal. word. }
     (* TODO: is there a good way of extracting this goal automatically? *)
-    replace (S (length proof.(PathProof.Id) - uint.nat (word.add loopIdx 1))) with
-      ((length proof.(PathProof.Id) - uint.nat loopIdx)%nat) by word.
+    replace (S (length proof.(pathProof.id) - uint.nat (word.add loopIdx 1))) with
+      ((length proof.(pathProof.id) - uint.nat loopIdx)%nat) by word.
     exists tr.
     split; [|done].
     rewrite (lookup_app_r _ _ _ _).
@@ -628,52 +560,33 @@ Proof.
   iEval (rewrite /for_inv); clear for_inv.
   iIntros "[H _]"; iNamed "H".
   wp_load.
-  wp_if_destruct; [by iApply "HΦ"|].
+  wp_if_destruct; [by iApply "HΦ"|]; clear err Heqb.
   iSimpl in "Herr_pred"; iNamed "Herr_pred".
-  wp_apply (wp_loadField with "Hptr_Digest");
-    iIntros "Hptr_Digest".
+  wp_apply (wp_loadField with "Hptr_digest");
+    iIntros "Hptr_digest".
   wp_load.
-  iMod (readonly_load with "Hro_sl_currHash") as (?) "Hsl_currHash".
-  wp_apply (wp_BytesEqual with "[$Hsl_currHash $HDigest]");
-    iIntros "[Hsl_currHash HDigest]".
-  wp_if_destruct; [by iApply "HΦ"|].
-  iEval (replace ((length proof.(PathProof.Id) - uint.nat sl_ChildHashes.(Slice.sz))%nat)
+  (* TODO: framing doesn't work here. $Hsl_currHash frames this persis thing twice. *)
+  wp_apply (wp_BytesEqual with "[Hdigest]"); [iFrame "#∗"|];
+    iIntros "[_ Hdigest]".
+  wp_if_destruct; [by iApply "HΦ"|]; rename Heqb into Heq_currHash.
+  iEval (replace ((length proof.(pathProof.id) - uint.nat sl_childHashes.(Slice.sz))%nat)
     with (0%nat) by word) in "Hpath_val".
-  iEval (rewrite drop_0 Heqb) in "Hpath_val".
+  iEval (rewrite drop_0 Heq_currHash) in "Hpath_val".
   by iApply "HΦ".
 Qed.
 
-Lemma wp_MembProofCheck sl_proof proof sl_id sl_val sl_digest (id val digest : list u8) :
+Lemma wp_CheckProof (proofTy : bool) sl_proof proof sl_id sl_val sl_digest (id val digest : list w8) :
   {{{
     "#Hproof" ∷ is_Slice3D sl_proof proof ∗
-    "Hid" ∷ own_slice_small sl_id byteT 1 id ∗
-    "Hval" ∷ own_slice_small sl_val byteT 1 val ∗
-    "Hdigest" ∷ own_slice_small sl_digest byteT 1 digest
+    "Hid" ∷ own_slice_small sl_id byteT (DfracOwn 1) id ∗
+    "Hval" ∷ own_slice_small sl_val byteT (DfracOwn 1) val ∗
+    "Hdigest" ∷ own_slice_small sl_digest byteT (DfracOwn 1) digest
   }}}
-  MembProofCheck (slice_val sl_proof) (slice_val sl_id) (slice_val sl_val) (slice_val sl_digest)
+  CheckProof #proofTy (slice_val sl_proof) (slice_val sl_id) (slice_val sl_val) (slice_val sl_digest)
   {{{
-    (err:u64), RET #err;
-    if bool_decide (err = 0) then
-      "#Hpath" ∷ is_path_val id (Some val) digest
-    else True%I
-  }}}.
-Proof.
-  iIntros (Φ) "H HΦ"; iNamed "H".
-  rewrite /MembProofCheck.
-  admit.
-Admitted.
-
-Lemma wp_NonmembCheck sl_proof proof sl_id sl_digest (id digest : list u8) :
-  {{{
-    "#Hproof" ∷ is_Slice3D sl_proof proof ∗
-    "Hid" ∷ own_slice_small sl_id byteT 1 id ∗
-    "Hdigest" ∷ own_slice_small sl_digest byteT 1 digest
-  }}}
-  NonmembProofCheck (slice_val sl_proof) (slice_val sl_id) (slice_val sl_digest)
-  {{{
-    (err:u64), RET #err;
-    if bool_decide (err = 0) then
-      "#Hpath" ∷ is_path_val id None digest
+    (err : bool), RET #err;
+    if negb err then
+      "H#Hpath" ∷ is_path_val id (if proofTy then Some val else None) digest
     else True%I
   }}}.
 Proof. Admitted.
